src/program_proof/tulip/program/replica/replica_fast_prepare.v
@@ -8,13 +8,13 @@ Section program.
   Context `{!heapGS Σ, !tulip_ghostG Σ}.
 
   Theorem wp_Replica__fastPrepare
-    rp (tsW : u64) pwrsS pwrsL pwrs gid rid γ α :
+    rp (tsW : u64) pwrsS pwrs gid rid γ α :
     let ts := uint.nat tsW in
     gid ∈ gids_all ->
     rid ∈ rids_all ->
     safe_txn_pwrs γ gid ts pwrs -∗
     know_tulip_inv γ -∗
-    {{{ own_dbmap_in_slice pwrsS pwrsL pwrs ∗ own_replica rp gid rid γ α }}}
+    {{{ own_dbmap_in_slice pwrsS pwrs ∗ own_replica rp gid rid γ α }}}
       Replica__fastPrepare #rp #tsW (to_val pwrsS) slice.nil
     {{{ (res : rpres), RET #(rpres_to_u64 res);
         own_replica rp gid rid γ α ∗ fast_prepare_outcome γ gid rid ts res
@@ -274,11 +274,11 @@ Section program.
   Qed.
 
   Theorem wp_Replica__FastPrepare
-    rp (tsW : u64) pwrsS pwrsL pwrs gid rid γ :
+    rp (tsW : u64) pwrsS pwrs gid rid γ :
     let ts := uint.nat tsW in
     safe_txn_pwrs γ gid ts pwrs -∗
     is_replica rp gid rid γ -∗
-    {{{ own_dbmap_in_slice pwrsS pwrsL pwrs }}}
+    {{{ own_dbmap_in_slice pwrsS pwrs }}}
       Replica__FastPrepare #rp #tsW (to_val pwrsS) slice.nil
     {{{ (res : rpres), RET #(rpres_to_u64 res);
         fast_prepare_outcome γ gid rid ts res
